A lot more work on shallow expressions. Most syntax is now available from basic expressions.

theories/core/utp_event.thy
@@ -23,6 +23,19 @@ abbreviation chan_type :: "'a CHANNEL \<Rightarrow> 'a UTYPE" where
 typedef 'a EVENT = "{(c::'a CHANNEL, v :: 'a). v : chan_type c}"
   by (auto)
 
+declare Rep_EVENT [simp]
+declare Rep_EVENT_inverse [simp]
+declare Abs_EVENT_inverse [simp]
+
+lemma Rep_EVENT_intro [intro]:
+  "Rep_EVENT x = Rep_EVENT y \<Longrightarrow> x = y"
+  by (auto simp add: Rep_EVENT_inject[THEN sym])
+
+abbreviation EV :: "NAME \<Rightarrow> 'a UTYPE \<Rightarrow> 'a \<Rightarrow> 'a EVENT" where
+"EV n t v \<equiv> Abs_EVENT ((n, t), v)"
+
+type_synonym 'a PEvent = "(NAME * 'a)"
+
 setup_lifting type_definition_EVENT
 
 lift_definition EVENT_channel :: "'a EVENT \<Rightarrow> 'a CHANNEL" is "fst"
@@ -30,5 +43,13 @@ lift_definition EVENT_channel :: "'a EVENT \<Rightarrow> 'a CHANNEL" is "fst"
 
 lift_definition EVENT_value :: "'a EVENT \<Rightarrow> 'a" is "snd"
   by simp
+
+lemma EVENT_channel_EV [simp]: 
+  "v : t \<Longrightarrow> EVENT_channel (EV n t v) = (n, t)"
+  by (auto simp add:EVENT_channel_def)
+
+lemma EVENT_value_EV [simp]:
+  "v : t \<Longrightarrow> EVENT_value (EV n t v) = v"
+  by (auto simp add:EVENT_value_def)
 
 end
