theories/core/utp_shallow_expr.thy
@@ -4,23 +4,30 @@
 (* Author: Simon Foster and Frank Zeyda, University of York (UK)              *)
 (******************************************************************************)
 
-header {* Shallow Expressions *}
+header {* Shallowly Embedded Polymorphic Expressions *}
 
 theory utp_shallow_expr
 imports 
   utp_expr
   "../tactics/utp_expr_tac"
+  "../laws/utp_subst_laws"
   utp_event
+  utp_rel
 begin
 
 default_sort type
+
+subsection {* Polymorphic constants *}
 
 consts 
   TypeU :: "'a itself \<Rightarrow> ('m :: VALUE) UTYPE"
   InjU  :: "'a \<Rightarrow> 'm :: VALUE"
   ProjU :: "'m :: VALUE \<Rightarrow> 'a"
 
-type_synonym 'a PEvent = "(NAME * 'a)"
+syntax
+  "_TYPEU" :: "type => logic"  ("(1TYPEU/(1'(_')))")
+
+translations "TYPEU('a)" == "CONST TypeU TYPE('a)"
 
 definition MkPEvent :: "'a PEvent \<Rightarrow> 'm :: EVENT_SORT" where
 "MkPEvent e = MkEvent (Abs_EVENT ((fst e, TypeU TYPE('a)), InjU (snd e)))"
@@ -50,26 +57,77 @@ defs (overloaded)
   TypeU_fset [simp]: "TypeU (x :: ('a fset) itself) \<equiv> FSetType (TypeU TYPE('a))"  
 
 text {* TypeUSound can be thought of as a two-parameter type class which stores
-        the properties of the above polymorphic constants *}
+        the properties of the above polymorphic constants, namely that the
+        given Isabelle type can be constructed under the given sort constraints *}
 
 definition TypeUSound :: "'a itself \<Rightarrow> 'm::VALUE itself \<Rightarrow> bool" where
-"TypeUSound a m = (\<forall> (x :: 'a). (InjU x :: 'm) :! TypeU a)"
+"TypeUSound a m \<longleftrightarrow> (\<forall> (x :: 'a). (InjU x :: 'm) :! TypeU a) \<and>
+                    (\<forall> (x :: 'a). (ProjU (InjU x :: 'm) = x))"
 
-lemma TypeUSound_bool [typing]: "TypeUSound TYPE(bool) TYPE('m :: BOOL_SORT)"
+syntax
+  "_TYPEUSOUND" :: "type \<Rightarrow> type => logic"  ("(1TYPEUSOUND/(1'(_, _')))")
+
+translations "TYPEUSOUND('a, 'm)" == "CONST TypeUSound TYPE('a) TYPE('m)"
+
+lemma TypeUSound_intro [intro]:
+  "\<lbrakk> \<And> (x :: 'a). (InjU x :: 'm) :! TYPEU('a)
+   ; \<And> (x :: 'a). (ProjU (InjU x :: 'm) = x) \<rbrakk> \<Longrightarrow>
+   TYPEUSOUND('a, 'm :: VALUE)"
+  by (simp add:TypeUSound_def)
+
+lemma TypeUSound_InjU_type [typing]:
+  fixes x :: "'a"
+  assumes "TYPEUSOUND('a, 'm :: VALUE)"
+  shows "(InjU x :: 'm) :! TYPEU('a)"
+  using assms by (auto simp add:TypeUSound_def)
+
+lemma TypeUSound_InjU_defined [defined]:
+  fixes x :: "'a"
+  assumes "TYPEUSOUND('a, 'm :: VALUE)"
+  shows "\<D> (InjU x :: 'm)"
+  by (auto intro:assms typing defined)
+
+lemma TypeUSound_InjU_inv [simp]:
+  fixes x :: "'a"
+  assumes "TYPEUSOUND('a, 'm :: VALUE)"
+  shows "ProjU (InjU x :: 'm) = x"
+  using assms by (auto simp add:TypeUSound_def)
+
+lemma TypeUSound_bool [typing]: "TYPEUSOUND(bool, 'm :: BOOL_SORT)"
   by (simp add:TypeUSound_def typing)
 
-lemma TypeUSound_int [typing]: "TypeUSound TYPE(int) TYPE('m :: INT_SORT)"
+lemma TypeUSound_int [typing]: "TYPEUSOUND(int, 'm :: INT_SORT)"
   by (simp add:TypeUSound_def typing)
 
 lemma TypeUSound_list [typing]: 
-  "\<lbrakk> (TypeU TYPE('a) :: 'm UTYPE) \<in> ListPerm; TypeUSound TYPE('a) TYPE('m :: LIST_SORT) \<rbrakk> 
-     \<Longrightarrow> TypeUSound TYPE('a list) TYPE('m)"
-  by (force intro:typing simp add:dcarrier_def TypeUSound_def)
+  "\<lbrakk> (TYPEU('a) :: 'm UTYPE) \<in> ListPerm; TYPEUSOUND('a, 'm) \<rbrakk> 
+     \<Longrightarrow> TYPEUSOUND('a list, 'm :: LIST_SORT)"
+  apply (auto simp add:dcarrier_def TypeUSound_def)
+  apply (rule typing, auto)
+  apply (subgoal_tac "set (map InjU x) \<subseteq> dcarrier (TYPEU('a) :: 'm UTYPE)")
+  apply (auto simp add:comp_def)
+done
 
 lemma TypeUSound_fset [typing]: 
-  "\<lbrakk> (TypeU TYPE('a) :: 'm UTYPE) \<in> FSetPerm; TypeUSound TYPE('a) TYPE('m :: FSET_SORT) \<rbrakk> 
-     \<Longrightarrow> TypeUSound TYPE('a fset) TYPE('m)"
-  by (force intro:typing simp add:dcarrier_def TypeUSound_def)
+  "\<lbrakk> (TYPEU('a) :: 'm UTYPE) \<in> FSetPerm; TYPEUSOUND('a, 'm) \<rbrakk> 
+     \<Longrightarrow> TYPEUSOUND('a fset, 'm :: FSET_SORT)"
+  apply (simp add:dcarrier_def TypeUSound_def)
+  apply (rule)
+  apply (clarify)
+  apply (rule typing)
+  apply (force)
+  apply (force)
+  apply (clarify)
+  apply (subgoal_tac "\<langle>InjU `\<^sub>f x\<rangle>\<^sub>f \<subseteq> dcarrier (TYPEU('a) :: 'm UTYPE)")
+  apply (auto simp add:image_def)
+done
+
+lemma TypeUSound_PEvent [typing]:
+  "\<lbrakk> (TYPEU('a) :: 'm UTYPE) \<in> EventPerm; TYPEUSOUND('a, 'm) \<rbrakk>
+     \<Longrightarrow> TYPEUSOUND('a PEvent, 'm :: EVENT_SORT)"
+  by (auto simp add:MkPEvent_def typing DestPEvent_def)
+
+subsection {* Polymorphic Expression Basic Syntax *}
 
 typedef ('a, 'm :: VALUE) WF_PEXPRESSION = "UNIV :: ('m WF_BINDING \<Rightarrow> 'a) set" ..
 
@@ -87,22 +145,84 @@ definition WF_PEXPRESSION_type ::
   "('a, 'm :: VALUE) WF_PEXPRESSION \<Rightarrow> 'm UTYPE" ("\<tau>\<^sub>*") where
 "WF_PEXPRESSION_type e = TypeU(TYPE('a))"
 
-definition "LitPE v = Abs_WF_PEXPRESSION (\<lambda> b. v)"
+definition LitPE :: "'a \<Rightarrow> ('a, 'm :: VALUE) WF_PEXPRESSION" where
+"LitPE v = Abs_WF_PEXPRESSION (\<lambda> b. v)"
 
 lemma EvalPE_LitPE [evale]:
   "\<lbrakk>LitPE v\<rbrakk>\<^sub>*b = v"
   by (simp add:LitPE_def)
 
-record ('a, 'm :: VALUE) PVAR = 
-  pvname  :: NAME
-  pvaux   :: bool
-  pvtype  :: "'a itself"
-  pvmodel :: "'m itself"
+lemma WF_PEXPRESSION_tau [typing]:
+  fixes v :: "('a, 'm :: VALUE) WF_PEXPRESSION"
+  shows "\<tau>\<^sub>*(v) = TypeU(TYPE('a))"
+  by (simp add:WF_PEXPRESSION_type_def)
 
-definition "myvar \<equiv> \<lparr> pvname = bName ''myvar'', pvaux = True, pvtype = TYPE(bool), pvmodel = TYPE('a :: BOOL_SORT) \<rparr>"
+definition pevar_compat :: 
+  "('a, 'm :: VALUE) WF_PEXPRESSION \<Rightarrow> 'm VAR \<Rightarrow> bool" (infix "\<rhd>\<^sub>*" 50) where
+"pevar_compat e x \<equiv> \<forall>b. InjU (\<lbrakk>e\<rbrakk>\<^sub>* b) \<rhd> x"
+
+typedef ('a, 'm :: VALUE) PVAR = "UNIV :: (NAME * bool) set"
+  by auto
+
+declare Rep_PVAR [simp]
+declare Rep_PVAR_inverse [simp]
+declare Abs_PVAR_inverse [simp]
+
+definition MkPVAR :: "NAME \<Rightarrow> bool \<Rightarrow> 'a itself \<Rightarrow> 'm itself \<Rightarrow> ('a, 'm :: VALUE) PVAR" where
+"MkPVAR n s a t = Abs_PVAR (n, s)"
+
+abbreviation pvname :: "('a, 'm :: VALUE) PVAR \<Rightarrow> NAME" where
+"pvname x \<equiv> fst (Rep_PVAR x)"
+
+abbreviation pvaux :: "('a, 'm :: VALUE) PVAR \<Rightarrow> bool" where
+"pvaux x \<equiv> snd (Rep_PVAR x)"
+
+lemma pvname_MkPVAR [simp]:
+  "pvname (MkPVAR n s a m) = n"
+  by (simp add:MkPVAR_def)
+
+lemma pvaux_MkPVAR [simp]:
+  "pvaux (MkPVAR n s a m) = s"
+  by (simp add:MkPVAR_def)
+
+definition pvundash :: "('a, 'm :: VALUE) PVAR \<Rightarrow> ('a, 'm :: VALUE) PVAR" where
+"pvundash v = Abs_PVAR (MkName (name_str (pvname v)) (dashes (pvname v) - 1) (subscript (pvname v)), pvaux v)"
+
+definition pvdash :: "('a, 'm :: VALUE) PVAR \<Rightarrow> ('a, 'm :: VALUE) PVAR" where
+"pvdash v = Abs_PVAR (MkName (name_str (pvname v)) (dashes (pvname v) + 1) (subscript (pvname v)), pvaux v)"
 
 definition PVAR_VAR :: "('a, 'm) PVAR \<Rightarrow> ('m :: VALUE) VAR" where
 "PVAR_VAR v = MkVar (pvname v) (TypeU TYPE('a)) (pvaux v)"
+
+definition VAR_PVAR :: "('m :: VALUE) VAR \<Rightarrow> ('a, 'm) PVAR" where
+"VAR_PVAR v = Abs_PVAR (name v, aux v)"
+
+lemma PVAR_VAR_inv [simp]: 
+  "VAR_PVAR (PVAR_VAR v) = v"
+  by (simp add:PVAR_VAR_def VAR_PVAR_def)
+
+lemma VAR_PVAR_inv [simp]: 
+  "vtype x = TYPEU('a) \<Longrightarrow> PVAR_VAR (VAR_PVAR x :: ('a, 'm :: VALUE) PVAR) = x"
+  apply (case_tac x)
+  apply (auto simp add:PVAR_VAR_def VAR_PVAR_def MkVar_def)
+done
+
+lemma PVAR_VAR_pvdash [simp]:
+  "PVAR_VAR (pvdash x) = dash (PVAR_VAR x)"
+  by (auto simp add:PVAR_VAR_def dash_def pvdash_def)
+
+lemma PVAR_VAR_compat [typing]:
+  fixes e :: "('a, 'm :: VALUE) WF_PEXPRESSION" 
+  and   x :: "('a, 'm) PVAR"
+  assumes "TYPEUSOUND('a, 'm)"
+  shows "e \<rhd>\<^sub>* PVAR_VAR x"
+  apply (auto simp add:pevar_compat_def PVAR_VAR_def assms typing var_compat_def)
+  apply (simp add:assms defined)
+done
+
+abbreviation "PUNDASHED     \<equiv> {x. PVAR_VAR x \<in> UNDASHED}"
+abbreviation "PDASHED       \<equiv> {x. PVAR_VAR x \<in> DASHED}"
+abbreviation "PDASHED_TWICE \<equiv> {x. PVAR_VAR x \<in> DASHED_TWICE}"
 
 definition "VarPE x = Abs_WF_PEXPRESSION (\<lambda> b. ProjU (\<langle>b\<rangle>\<^sub>b x))"
 
@@ -111,6 +231,10 @@ abbreviation PVarPE :: "('a, 'm :: VALUE) PVAR \<Rightarrow> ('a, 'm) WF_PEXPRES
 
 lemma EvalPE_VarPE [evale]:
   "\<lbrakk>VarPE x\<rbrakk>\<^sub>*b = ProjU (\<langle>b\<rangle>\<^sub>b x)"
+  by (simp add:VarPE_def)
+
+lemma EvalPE_PVarPE [evale]:
+  "\<lbrakk>PVarPE x\<rbrakk>\<^sub>*b = ProjU (\<langle>b\<rangle>\<^sub>b (PVAR_VAR x))"
   by (simp add:VarPE_def)
 
 definition "Op1PE f u = Abs_WF_PEXPRESSION (\<lambda> b. f (Rep_WF_PEXPRESSION u b))"
@@ -130,6 +254,8 @@ definition "Op3PE f u v w = Abs_WF_PEXPRESSION (\<lambda> b. f (Rep_WF_PEXPRESSI
 lemma EvalPE_Op3PE [evale]:
   "\<lbrakk>Op3PE f u v w\<rbrakk>\<^sub>*b = f (\<lbrakk>u\<rbrakk>\<^sub>*b) (\<lbrakk>v\<rbrakk>\<^sub>*b) (\<lbrakk>w\<rbrakk>\<^sub>*b)"
   by (simp add:Op3PE_def)
+
+abbreviation "EqualPE \<equiv> Op2PE (op =)"
 
 definition PExprE :: "('a, 'm :: VALUE) WF_PEXPRESSION \<Rightarrow> 'm WF_EXPRESSION" where
 "PExprE f = Abs_WF_EXPRESSION (InjU \<circ> Rep_WF_PEXPRESSION f)"
@@ -154,29 +280,12 @@ lemma EvalE_PExprE [evale]:
 
 lemma PExprE_type [typing]:
   fixes e :: "('a, 'm :: VALUE) WF_PEXPRESSION" 
-  assumes "TypeUSound TYPE('a) TYPE('m)"
-  shows "PExprE e :\<^sub>e \<tau>\<^sub>* e"
+  assumes "TypeUSound TYPE('a) TYPE('m)" 
+  and "t = \<tau>\<^sub>* e"
+  shows "PExprE e :\<^sub>e t"
   apply (simp add: etype_rel_def PExprE_rep_eq assms WF_PEXPRESSION_type_def)
   apply (metis TypeUSound_def assms dtype_type)
 done
-
-definition SubstPE :: 
-"('a, 'm :: VALUE) WF_PEXPRESSION \<Rightarrow> 
- ('b, 'm) WF_PEXPRESSION \<Rightarrow> 
- 'm VAR \<Rightarrow> 
- ('a, 'm) WF_PEXPRESSION" where
-"SubstPE f v x = Abs_WF_PEXPRESSION (\<lambda> b. \<lbrakk>f\<rbrakk>\<^sub>* (b(x :=\<^sub>b InjU (\<lbrakk>v\<rbrakk>\<^sub>* b))))"
-
-lemma EvalPE_SubstPE [evale]:
-  "\<lbrakk>SubstPE e v x\<rbrakk>\<^sub>*b = \<lbrakk>e\<rbrakk>\<^sub>* (b(x :=\<^sub>b InjU (\<lbrakk>v\<rbrakk>\<^sub>* b)))"
-  by (simp add:SubstPE_def)
-
-abbreviation PSubstPE :: 
-"('a, 'm :: VALUE) WF_PEXPRESSION \<Rightarrow> 
- ('b, 'm) WF_PEXPRESSION \<Rightarrow> 
- ('b, 'm) PVAR \<Rightarrow> 
- ('a, 'm) WF_PEXPRESSION" where
-"PSubstPE f v x \<equiv> SubstPE f v (PVAR_VAR x)"
 
 subsection {* Boolean Expressions *}
 
@@ -265,5 +374,171 @@ lemma FUnionPE_type:
   "\<tau>\<^sub>* (FUnionPE (xs :: ('a fset, 'm :: FSET_SORT) WF_PEXPRESSION) ys) 
    = FSetType (TypeU TYPE('a))"
   by (simp add: WF_PEXPRESSION_type_def)
+
+subsection {* Action Expressions *}
+
+abbreviation EventPE ::
+  "NAME \<Rightarrow> ('a, 'm :: EVENT_SORT) WF_PEXPRESSION 
+        \<Rightarrow> ('a PEvent, 'm) WF_PEXPRESSION" where
+"EventPE n v \<equiv> Op1PE (\<lambda> v. (n, v)) v"
+
+subsection {* Renaming *}
+
+definition RenamePE ::
+  "('a, 'm :: VALUE) WF_PEXPRESSION \<Rightarrow>
+   'm VAR_RENAME \<Rightarrow>
+   ('a, 'm) WF_PEXPRESSION" where
+"RenamePE e ss = Abs_WF_PEXPRESSION (\<lbrakk>e\<rbrakk>\<^sub>* \<circ> (RenameB (inv\<^sub>s ss)))"
+
+lemma EvalPE_RenamePE [evale]:
+  "\<lbrakk>RenamePE e ss\<rbrakk>\<^sub>* = \<lbrakk>e\<rbrakk>\<^sub>* \<circ> (RenameB (inv\<^sub>s ss))"
+  by (simp add:RenamePE_def)
+
+definition Rep_VAR_RENAME_poly :: 
+  "'m VAR_RENAME \<Rightarrow> ('a, 'm :: VALUE) PVAR \<Rightarrow> ('a, 'm) PVAR" where
+"Rep_VAR_RENAME_poly ss x \<equiv> VAR_PVAR (Rep_VAR_RENAME ss (PVAR_VAR x))"
+
+notation Rep_VAR_RENAME_poly ("\<langle>_\<rangle>\<^sub>s\<^sub>*")
+
+lemma PVAR_VAR_vtype [simp]:
+  "vtype (PVAR_VAR (x :: ('a, 'm :: VALUE) PVAR)) = TYPEU('a)"
+  by (simp add:PVAR_VAR_def)
+
+lemma PVAR_VAR_RENAME [simp]: 
+  "PVAR_VAR (\<langle>ss\<rangle>\<^sub>s\<^sub>* x) = \<langle>ss\<rangle>\<^sub>s (PVAR_VAR x)"
+  by (simp add:Rep_VAR_RENAME_poly_def)
+
+lemma RenamePE_PVarPE [urename]:
+  "RenamePE (VarPE x) ss = VarPE (\<langle>ss\<rangle>\<^sub>s x)"
+  by (auto simp add:evale)
+
+(*
+lemma RenamePE_PVarPE [urename]:
+  "RenamePE (PVarPE x) ss = PVarPE (\<langle>ss\<rangle>\<^sub>s\<^sub>* x)"
+  apply (simp add:urename)
+  by (auto simp add:evale)
+*)
+
+lemma RenamePE_LitPE [urename]:
+  "RenamePE (LitPE v) ss = LitPE v"
+  by (auto simp add:evale)
+
+lemma RenamePE_Op1PE [urename]:
+  "RenamePE (Op1PE f v) ss = Op1PE f (RenamePE v ss)"
+  by (auto simp add:evale)
+
+lemma RenamePE_Op2PE [urename]:
+  "RenamePE (Op2PE f u v) ss = Op2PE f (RenamePE u ss) (RenamePE v ss)"
+  by (auto simp add:evale)
+
+lemma RenamePE_Op3PE [urename]:
+  "RenamePE (Op3PE f u v w) ss = Op3PE f (RenamePE u ss) (RenamePE v ss) (RenamePE w ss)"
+  by (auto simp add:evale)
+
+subsection {* Substitution *}
+
+definition SubstPE :: 
+"('a, 'm :: VALUE) WF_PEXPRESSION \<Rightarrow> 
+ ('b, 'm) WF_PEXPRESSION \<Rightarrow> 
+ 'm VAR \<Rightarrow> 
+ ('a, 'm) WF_PEXPRESSION" where
+"SubstPE f v x = Abs_WF_PEXPRESSION (\<lambda> b. \<lbrakk>f\<rbrakk>\<^sub>* (b(x :=\<^sub>b InjU (\<lbrakk>v\<rbrakk>\<^sub>* b))))"
+
+abbreviation PSubstPE :: 
+"('a, 'm :: VALUE) WF_PEXPRESSION \<Rightarrow> 
+ ('b, 'm) WF_PEXPRESSION \<Rightarrow> 
+ ('b, 'm) PVAR \<Rightarrow> 
+ ('a, 'm) WF_PEXPRESSION" where
+"PSubstPE f v x \<equiv> SubstPE f v (PVAR_VAR x)"
+
+lemma EvalPE_SubstPE [evale]:
+  "\<lbrakk>SubstPE e v x\<rbrakk>\<^sub>*b = \<lbrakk>e\<rbrakk>\<^sub>* (b(x :=\<^sub>b InjU (\<lbrakk>v\<rbrakk>\<^sub>* b)))"
+  by (simp add:SubstPE_def)
+
+lemma SubstPE_VarPE [usubst]:
+  fixes v :: "('a, 'm :: VALUE) WF_PEXPRESSION"
+  assumes "v \<rhd>\<^sub>* x" "TYPEUSOUND('a, 'm)"
+  shows "SubstPE (VarPE x) v x = v"
+  using assms by (auto simp add:evale pevar_compat_def)
+
+lemma PSubstPE_PVarPE [usubst]:
+  fixes v :: "('a, 'm :: VALUE) WF_PEXPRESSION"
+  assumes "TYPEUSOUND('a, 'm)"
+  shows "PSubstPE (PVarPE x) v x = v"
+  using assms by (simp add:usubst typing)
+
+lemma SubstPE_LitPE [usubst]:
+  "SubstPE (LitPE v) x e = LitPE v"
+  by (auto simp add:evale)
+
+lemma SubstPE_Op1PE [usubst]:
+  "SubstPE (Op1PE f v) x e = Op1PE f (SubstPE v x e)"
+  by (auto simp add:evale)
+
+lemma SubstPE_Op2PE [usubst]:
+  "SubstPE (Op2PE f u v) e x = Op2PE f (SubstPE u e x) (SubstPE v e x)"
+  by (auto simp add:evale)
+
+lemma SubstPE_Op3PE [usubst]:
+  "SubstPE (Op3PE f u v w) e x= Op3PE f (SubstPE u e x) (SubstPE v e x) (SubstPE w e x)"
+  by (auto simp add:evale)
+
+subsection {* Parser *}
+
+abbreviation "okay \<equiv> MkPVAR (bName ''okay'') True TYPE(bool) TYPE('m :: BOOL_SORT)"
+
+lemma [closure]: "PVAR_VAR okay \<in> UNDASHED"
+  apply (simp add:PVAR_VAR_def)
+  apply (metis MkPlain_UNDASHED MkPlain_def)
+done
+
+
+nonterminal pexpr and pexprs
+
+syntax
+  "_pexprs"             :: "[pexpr, pexprs] => pexprs" ("_,/ _")
+  ""                    :: "pexpr => pexprs" ("_")
+  "_pexpr_brack"        :: "pexpr \<Rightarrow> pexpr" ("'(_')")
+  "_expr_quote"         :: "pexpr \<Rightarrow> 'a WF_EXPRESSION" ("(1|_|)")
+  "_pexpr_quote"        :: "pexpr \<Rightarrow> ('a, 'm) WF_PEXPRESSION" ("(1\<parallel>_\<parallel>)")
+  "_pexpr_true"         :: "pexpr" ("true")
+  "_pexpr_false"        :: "pexpr" ("false")
+  "_pexpr_int"          :: "int \<Rightarrow> pexpr" ("_")
+  "_pexpr_evar"         :: "('a, 'm) PVAR \<Rightarrow> pexpr" ("$_" [999] 999)
+  "_pexpr_list"         :: "pexprs \<Rightarrow> pexpr" ("\<langle>_\<rangle>")
+  "_pexpr_list_nil"     :: "pexpr" ("\<langle>\<rangle>")
+  "_pexpr_list_append"  :: "pexpr \<Rightarrow> pexpr \<Rightarrow> pexpr" (infixr "^" 65)
+  "_pexpr_fset"         :: "pexprs \<Rightarrow> pexpr" ("{_}")
+  "_pexpr_fset_empty"   :: "pexpr" ("{}")
+  "_pexpr_fset_union"   :: "pexpr \<Rightarrow> pexpr \<Rightarrow> pexpr" (infixl "\<union>" 65)
+  "_pexpr_fset_inter"   :: "pexpr \<Rightarrow> pexpr \<Rightarrow> pexpr" (infixl "\<inter>" 70)
+
+translations
+  "_pexpr_brack e"             => "e"
+  "_expr_quote e"              => "CONST PExprE e"
+  "_pexpr_quote e"             => "e"
+  "_pexpr_true"                == "CONST TruePE"
+  "_pexpr_false"               == "CONST FalsePE"
+  "_pexpr_int x"               == "CONST IntPE x"
+  "_pexpr_evar x"              == "CONST PVarPE x"
+  "_pexpr_list_nil"            == "CONST NilPE"
+  "_pexpr_list_append e f"     == "CONST ConcatPE e f"
+  "_pexpr_list (_pexprs x xs)" == "CONST ConsPE x (_pexpr_list xs)"
+  "_pexpr_list x"              == "CONST ConsPE x (CONST NilPE)"
+  "_pexpr_fset (_pexprs x xs)" == "CONST FInsertPE x (_pexpr_fset xs)"
+  "_pexpr_fset x" == "CONST FInsertPE x CONST FEmptyPE"
+  "_pexpr_fset_empty" == "CONST FEmptyPE"
+  "_pexpr_fset_union xs ys" == "CONST FUnionPE xs ys"
+  "_pexpr_fset_inter xs ys" == "CONST FInterPE xs ys"
+
+class MY_SORT = LIST_SORT + INT_SORT + BOOL_SORT +
+  assumes IntType_ListPerm [typing]: "IntType \<in> ListPerm"
+
+abbreviation "tr \<equiv> MkPVAR (bName ''tr'') True TYPE(int list) TYPE('m :: MY_SORT)"
+
+lemma "|\<langle>1,2\<rangle> ^ \<langle>3,4\<rangle> ^ $tr| = |\<langle>1,2,3,4\<rangle> ^ $tr|"
+  by (simp add:evale typing)
+ 
+term "|{1,3} \<union> {1,2}|"
 
 end
