theories/core/utp_sorts.thy
@@ -183,12 +183,12 @@ end
 subsection {* Name Sort *}
 
 class NAME_SORT = VALUE +
-  fixes MkName :: "NAME \<Rightarrow> 'a"
-  fixes DestName :: "'a \<Rightarrow> NAME"
-  fixes NameType  :: "'a UTYPE"
-  assumes Inverse [simp] : "DestName (MkName b) = b"
-  and     MkName_dcarrier: "dcarrier NameType = range MkName"
-  and     NameType_monotype [typing]: "monotype NameType"
+  fixes MkNm :: "NAME \<Rightarrow> 'a"
+  fixes DestNm :: "'a \<Rightarrow> NAME"
+  fixes NmType  :: "'a UTYPE"
+  assumes Inverse [simp] : "DestNm (MkNm b) = b"
+  and     MkNm_dcarrier: "dcarrier NmType = range MkNm"
+  and     NmType_monotype [typing]: "monotype NmType"
 
 subsection {* Event Sort *}
 
@@ -196,9 +196,24 @@ class EVENT_SORT = VALUE +
   fixes MkEvent :: "'a EVENT \<Rightarrow> 'a"
   and   DestEvent :: "'a \<Rightarrow> 'a EVENT"
   and   EventType :: "'a UTYPE"
-  assumes Inverse [simp] : "DestEvent (MkEvent b) = b"
-  and     MkEvent_dcarrier: "dcarrier EventType = range MkEvent"
+  and   EventPerm :: "'a UTYPE set"
+
+  assumes Inverse [simp] : 
+    "\<lbrakk> a \<in> EventPerm; EVENT_value v : a \<rbrakk> \<Longrightarrow> DestEvent (MkEvent v) = v"
+  and     MkEvent_dcarrier: 
+    "dcarrier EventType = MkEvent ` {EV n t v | n t v. t \<in> EventPerm \<and> v :! t} "
   and     EventType_monotype [typing]: "monotype EventType"
+begin
+
+lemma MkEvent_defined [defined] : 
+  "\<lbrakk> t \<in> EventPerm; v :! t \<rbrakk> \<Longrightarrow> \<D> (MkEvent (EV n t v))"
+  by (metis (lifting, mono_tags) MkEvent_dcarrier dcarrier_defined imageI mem_Collect_eq)
+
+lemma MkEvent_dtype [typing]: 
+  "\<lbrakk> t \<in> EventPerm; v :! t \<rbrakk> \<Longrightarrow> MkEvent (EV n t v) :! EventType"
+  by (metis (lifting, mono_tags) MkEvent_dcarrier dcarrier_dtype imageI mem_Collect_eq)
+
+end
 
 subsection {* Boolean Sort *}
 
